vera/VerilogToSMTCorrect.v
@@ -1,54 +1,116 @@
 From vera Require Import Common.
+From vera Require Import Decidable.
 From vera Require Import Tactics.
 From vera Require Import VerilogToSMT.
 From vera Require Import SMT.
 From vera Require Import VerilogSemantics.
+From vera Require Import Verilog.
 Import CombinationalOnly.
 
 From Coq Require List.
 
 From Equations Require Import Equations.
 
-Theorem verilog_to_smt_map_match tag start v smt :
+Lemma assign_vars_vars start vars :
+  List.map fst (assign_vars start vars) = vars.
+Proof.
+  revert start.
+  induction vars; intros;
+    simp assign_vars in *; cbn in *.
+  - reflexivity.
+  - rewrite IHvars. reflexivity.
+Qed.
+
+Lemma assign_vars_smtname_start start vars :
+  List.Forall (fun n => n >= start) (List.map snd (assign_vars start vars)).
+Proof.
+  revert start.
+  induction vars;
+    intros; simp assign_vars in *; cbn in *;
+    constructor.
+  - lia.
+  - specialize (IHvars (S start)).
+    revert IHvars.
+    eapply List.Forall_impl.
+    lia.
+Qed.
+
+Lemma assign_vars_smtname_nodup start vars :
+  List.NoDup (List.map snd (assign_vars start vars)).
+Proof.
+  revert start.
+  induction vars; intros; simp assign_vars in *; cbn in *;
+    constructor.
+  - intro contra.
+    pose proof (assign_vars_smtname_start (S start) vars).
+    eapply List.Forall_forall in H; try eassumption.
+    lia.
+  - eapply IHvars.
+Qed.
+
+Lemma mk_bijection_smt_map_match tag start v m :
+  mk_bijection tag (assign_vars start (Verilog.modVariables v)) = inr m ->
+  SMT.match_map_verilog tag m v.
+Proof.
+  Opaque VerilogSMTBijection.lookup_left.
+  unfold SMT.match_map_verilog.
+  replace (variable_names (Verilog.modVariables v)) with (variable_names (List.map fst (assign_vars start (Verilog.modVariables v))))
+    by now rewrite assign_vars_vars.
+  remember (assign_vars start (Verilog.modVariables v)) as assignment.
+  epose proof (assign_vars_smtname_nodup _ _) as Hnodup;
+    rewrite <- Heqassignment in Hnodup.
+  clear v start Heqassignment.
+  generalize dependent Hnodup.
+  generalize dependent m.
+  induction assignment; intros * ? Hbijection.
+  - simp mk_bijection in *. inv Hbijection.
+    split; intros H; cbn in *; solve_by_inverts 2%nat.
+  - unfold variable_names.
+    destruct a as [var smtName].
+    simp mk_bijection in Hbijection; inv Hbijection; autodestruct.
+    intros. split; intros H.
+    + destruct H as [smtName' H].
+      cbn.
+      cbn in H.
+      repeat match goal with
+      | [ H: context[sumbool_rec _ _ _  (?d ?a ?b)] |- _ ] =>
+          destruct (d a b); cbn in H; subst; try (congruence || contradiction)
+      | [ |- context[sumbool_rec _ _ _  (?d ?a ?b)] ] =>
+          destruct (d a b); cbn in H; subst; try (congruence || contradiction)
+      end.
+      * eauto.
+      * right.
+        unfold variable_names in IHassignment.
+        eapply IHassignment.
+        -- now inv Hnodup.
+        -- reflexivity.
+        -- eauto.
+    + cbn.
+      repeat match goal with
+      | [ H: context[sumbool_rec _ _ _  (?d ?a ?b)] |- _ ] =>
+          destruct (d a b); cbn in H; subst; try (congruence || contradiction)
+      | [ |- context[sumbool_rec _ _ _  (?d ?a ?b)] ] =>
+          destruct (d a b); cbn; subst; try (congruence || contradiction)
+      end.
+      * eauto.
+      * inv Hnodup. inv H; eapply IHassignment; eauto.
+        cbn in *. contradiction.
+Qed.
+
+Lemma verilog_to_smt_map_match tag start v smt :
   verilog_to_smt tag start v = inr smt ->
   SMT.match_map_verilog tag (SMT.nameMap smt) v.
 Proof.
-  unfold SMT.match_map_verilog.
   intros.
   funelim (verilog_to_smt tag start v);
     simp verilog_to_smt in *;
     try rewrite Heq in *;
     simpl in *;
     try discriminate.
-  autodestruct_eqn E.
-  simpl.
-  Set Nested Proofs Allowed.
-  Lemma ind : forall vars tag var_start verilogName,
-             (exists smtName : nat,
-                 VerilogSMTBijection.lookup_left
-                   (List.map (fun '(vname, smtname, _) => (tag, vname, smtname))
-                      (transfer_vars var_start vars))
-                   (tag, verilogName) = Some smtName) <->
-               List.In verilogName
-                 (VerilogSemantics.CombinationalOnly.variable_names vars).
-  Proof.
-    induction vars;
-      intros; simpl in *;
-      [ firstorder; discriminate | ].
-    destruct a; simpl in *.
-    destruct (TaggedName.dec_eq_tag tag tag); try contradiction.
-    destruct (dec (verilogName = varName));
-      simpl in *; subst;
-      firstorder.
-    - eauto.
-    - eauto.
-    - right. rewrite <- IHvars. eauto.
-    - subst. contradiction.
-    - rewrite IHvars. assumption.
-  Qed.
-  Unset Nested Proofs Allowed.
-  apply ind.
+  autodestruct_eqn E. cbn.
+  eauto using mk_bijection_smt_map_match.
 Qed.
+
 
 Theorem verilog_to_smt_correct tag start v smt :
   verilog_to_smt tag start v = inr smt ->
@@ -56,8 +118,7 @@ Theorem verilog_to_smt_correct tag start v smt :
     (SMT.query smt)
     (fun ρ => valid_execution v (SMT.execution_of_valuation tag (SMT.nameMap smt) ρ)).
 Proof.
-  intros.
-  funelimverilog_to_smt tag start v
+Admitted.
 
 Lemma verilog_to_smt_only_tag t n v s :
   verilog_to_smt t n v = inr s ->
